Matroid/Modular.lean
@@ -415,28 +415,174 @@ theorem SkewFamily.cls_skewFamily (h : M.SkewFamily Xs) : M.SkewFamily (fun i �
   rwa [← (h.modularFamily.modularPair i j).inter_cl_eq]
 
 theorem skewFamily_iff_exist_bases : M.SkewFamily Xs ↔
-    ∃ (Is : ι → Set α), M.Indep (⋃ i : ι, Is i) ∧ univ.PairwiseDisjoint Is ∧
+    ∃ (Is : ι → Set α), univ.PairwiseDisjoint Is ∧ M.Basis (⋃ i : ι, Is i) (⋃ i : ι, Xs i) ∧
       ∀ i, M.Basis (Is i) (Xs i) := by
-  refine ⟨fun h ↦ ?_, fun ⟨Is, hIs, hdj, hb⟩ ↦ ⟨hIs.modularFamily fun i ↦ ?_, fun i j hij ↦ ?_⟩⟩
+  refine ⟨fun h ↦ ?_,
+    fun ⟨Is, hdj, hIs, hb⟩ ↦ ⟨hIs.indep.modularFamily fun i ↦ ?_, fun i j hij ↦ ?_⟩⟩
   · obtain ⟨B, hB⟩ := h.modularFamily
-    exact ⟨fun i ↦ Xs i ∩ B, hB.indep.subset (iUnion_subset fun _ ↦ inter_subset_right _ _),
-      h.pairwiseDisjoint_inter_of_indep hB.base.indep, hB.basis_inter⟩
-  · rw [hIs.inter_basis_cl_iff_subset_cl_inter]
+    refine ⟨_, ?_, ?_, hB.basis_inter⟩
+    · exact h.disjoint_of_indep_subsets (fun i ↦ inter_subset_left _ _)
+        (fun i ↦ hB.indep.inter_left _)
+    rw [← iUnion_inter]
+    exact hB.basis_iUnion
+  · rw [hIs.indep.inter_basis_cl_iff_subset_cl_inter]
     exact (hb i).subset_cl.trans (M.cl_subset_cl (subset_inter (hb i).subset (subset_iUnion _ _)))
   refine (inter_subset_inter (M.subset_cl _ (hb i).subset_ground)
     (M.subset_cl _ (hb j).subset_ground)).trans ?_
-  rw [← (hb i).cl_eq_cl, ← (hb j).cl_eq_cl, ← (hIs.subset _).cl_inter_eq_inter_cl,
+  rw [← (hb i).cl_eq_cl, ← (hb j).cl_eq_cl, ← (hIs.indep.subset _).cl_inter_eq_inter_cl,
     Disjoint.inter_eq <| hdj (mem_univ i) (mem_univ j) hij]
   exact union_subset (subset_iUnion _ _) (subset_iUnion _ _)
 
+theorem SkewFamily.iUnion_indep_subset_indep (h : M.SkewFamily Xs) (hIX : ∀ i, Is i ⊆ Xs i)
+    (hIs : ∀ i, M.Indep (Is i)) : M.Indep (⋃ i, Is i) := by
+  choose Js hJs using fun i ↦ (hIs i).subset_basis_of_subset (hIX i)
+  refine Indep.subset ?_ <| iUnion_mono (fun i ↦ (hJs i).2)
 
--- theorem SkewFamily.iUnion_indep_subset_indep (h : M.SkewFamily Xs) (hIX : ∀ i, Is i ⊆ Xs i)
---     (hIs : ∀ i, M.Indep (Is i)) : M.Indep (⋃ i, Is i) := by
---   obtain ⟨Js, hJ, hdj, hJs⟩ := skewFamily_iff_exist_bases.1 h
---   rw [indep_iff_forall_subset_not_circuit]
---   intro C hCss hC
---   obtain ⟨e, heC⟩ := hC.nonempty
---   obtain ⟨_, ⟨i₀,rfl⟩, hei₀ : e ∈ Is i₀⟩ := hCss heC
+  obtain ⟨J, hJ⟩ := M.exists_basis (⋃ i, Js i) sorry
+
+  by_contra hcon
+  have ex_i : ∃ i e, e ∈ (Js i) \ J
+  · sorry
+
+  obtain ⟨i₀, e, hei₀, heJ⟩ := ex_i
+
+  obtain ⟨Ks, hdj, hKs, huKs⟩ := skewFamily_iff_exist_bases.1 h
+
+  have hssE : Js i₀ ∪ (⋃ i ∈ ({i₀}ᶜ : Set ι), Ks i) ⊆ M.E
+  · sorry
+
+  obtain ⟨K', hK', hss⟩ := (hJs i₀).1.indep.subset_basis_of_subset sorry hssE
+
+  have hK'' : ∀ i, i ≠ i₀ → Ks i ⊆ K'
+  · intro i hne f hf
+
+    by_contra hfK'
+    refine hfK' <| hK'.mem_of_insert_indep (Or.inr <| mem_biUnion hne hf) ?_
+    rw [hK'.indep.insert_indep_iff_of_not_mem hfK', mem_diff,
+      and_iff_right ((huKs i).indep.subset_ground hf)]
+    refine not_mem_subset ?_ <| hKs.indep.not_mem_cl_diff_of_mem (mem_iUnion.2 ⟨i,hf⟩)
+
+    rw [hK'.cl_eq_cl, M.cl_subset_cl_iff_subset_cl]
+
+
+
+    simp only [mem_compl_iff, mem_singleton_iff, mem_iUnion, not_exists, union_subset_iff,
+      iUnion_subset_iff]
+    refine ⟨?_, fun j hjne ↦ ?_⟩
+    · refine (hJs i₀).1.subset.trans ((huKs i₀).subset_cl.trans (M.cl_subset_cl ?_))
+      refine subset_diff_singleton (subset_iUnion Ks i₀) (fun hKsi₀ ↦ ?_)
+      exact (hdj (mem_univ i) (mem_univ i₀) hne).ne_of_mem hf hKsi₀ rfl
+
+
+    sorry
+    -- refine hK'.cl_subset_c.trans ?_
+
+
+  have he' : e ∈ M.cl (K' \ {e})
+  · refine mem_of_mem_of_subset (hJ.subset_cl (mem_iUnion_of_mem _ hei₀)) ?_
+    rw [cl_subset_cl_iff_subset_cl]
+    rintro f hf
+    obtain ⟨i, hfi⟩ := mem_iUnion.1 (hJ.subset hf)
+    obtain (rfl | hi) := eq_or_ne i₀ i
+    · apply M.subset_cl (K' \ {e}) ((diff_subset _ _).trans hK'.indep.subset_ground)
+      exact ⟨hss hfi, fun (h : f = e) ↦ heJ <| h ▸ hf⟩
+    refine mem_of_mem_of_subset ((hJs i).1.subset.trans (huKs i).subset_cl hfi) (M.cl_subset_cl ?_)
+    refine subset_diff_singleton (hK'' i hi.symm) (fun heK ↦ ?_)
+    apply Loop.not_nonloop <| h.loop_of_mem_inter hi ⟨(hJs i₀).1.subset hei₀, (huKs i).subset heK⟩
+    exact (hK'.indep.subset hss).nonloop_of_mem hei₀
+
+--   exact hK'.indep.not_mem_cl_diff_of_mem (hss hei₀) he'
+      -- refine mem_of_mem_of_subset ?_ (M.subset_cl ?_ ((diff_subset _ _).trans hK'.subset_ground)))
+
+    -- rw [hJ.cl_eq_cl, cl_subset_cl_iff_subset_cl hJ.subset_ground, iUnion_subset_iff]
+    -- intro i
+    -- obtain (rfl | hi) := eq_or_ne i₀ i
+    -- · refine subset_trans ?_ (hJ.subset_cl.trans ?_)
+
+  -- have hJ₀K' : e ∈ M.cl
+  -- ·
+
+
+  -- have ex_i : ∃ i, I ∩ (Is i) ⊂ Is i
+  -- · by_contra' h
+  --   refine hcon (hI.indep.subset (iUnion_subset fun i ↦ ?_))
+  --   exact (inter_subset_right I (Is i)).eq_or_ssubset.elim inter_eq_right.1 (fun h' ↦ (h i h').elim)
+  -- obtain ⟨i₀, hi₀ss⟩ := ex_i
+
+
+
+
+
+  --
+
+  -- obtain ⟨J₀, hJ₀, hssJ₀⟩ := (hI.indep.inter_right (Is i₀)).subset_basis_of_subset
+  --   (subset_union_left _ (Ks i₀)) (union_subset
+  --     ((inter_subset_left _ _).trans hI.indep.subset_ground) (huKs i₀).indep.subset_ground)
+
+  -- -- This is a good test for `aesop_mat`.
+  -- have hssE : J₀ ∪ (⋃ i ∈ ({i₀}ᶜ : Set ι), Ks i) ⊆ M.E
+  -- · refine union_subset hJ₀.indep.subset_ground ?_
+  --   simp only [mem_compl_iff, mem_singleton_iff, iUnion_subset_iff]
+  --   exact fun i _ ↦ (huKs i).indep.subset_ground
+
+  -- obtain ⟨K',hK',hss⟩ := hJ₀.indep.subset_basis_of_subset (subset_union_left _ _) hssE
+
+
+  -- have hK'' : M.Basis K'
+
+
+
+
+  -- have hKd := biUnion_subset_biUnion_left (subset_univ ({i₀}ᶜ : Set ι)) (t := Ks)
+  -- rw [biUnion_univ] at hKd
+  -- obtain ⟨K', hK', hss⟩ :=
+  --   (hKs.indep.subset hKd).subset_basis_of_subset (subset_union_left _ J₀)
+  --     (union_subset (hKd.trans hKs.indep.subset_ground) hJ₀.indep.subset_ground)
+
+
+
+
+
+
+    -- rw [← inter_eq_right, subset_antisymm_iff, and_iff_right (inter_subset_right _ _),
+    --   subset_iff_ssubset_or_eq]
+  -- choose Js hJs using fun i ↦ (hIs i).subset_basis_of_subset (hIX i)
+  -- refine Indep.subset ?_ <| iUnion_mono (fun i ↦ (hJs i).2)
+  -- obtain ⟨Ks, hdj, hKs, huKs⟩ := skewFamily_iff_exist_bases.1 h
+  -- obtain ⟨J, hJ⟩ := M.exists_basis (⋃ i, Js i)
+  --   (iUnion_subset (fun i ↦ (hJs i).1.indep.subset_ground))
+  -- obtain (rfl | hss) := hJ.subset.eq_or_ssubset
+  -- · exact hJ.indep
+  -- obtain ⟨e, ⟨_,⟨i₀,rfl⟩, (hi₀ : e ∈ Js i₀)⟩, heJs⟩ := exists_of_ssubset hss
+  -- obtain ⟨J', hJ', hss⟩  := (hJ.indep.inter_left (Xs i₀)).subset_basis_of_subset
+  --   (subset_union_left _ (⋃ i ∈ ({i₀}ᶜ : Set ι), Ks i)) sorry
+  -- have hJ'b : M.Basis J' (⋃ i, Xs i) := sorry
+
+
+
+
+
+  -- have
+
+
+  -- have hJX : M.Basis J (⋃ i, Xs i)
+  -- · refine hJ.basis_of_cl_eq_cl (hJ.subset.trans (iUnion_mono (fun i ↦ (hJs i).1.subset))) ?_
+  --   simp_rw [← M.cl_iUnion_cl_eq_cl_iUnion Js,
+  --     fun i ↦ (hJs i).1.cl_eq_cl, M.cl_iUnion_cl_eq_cl_iUnion]
+
+
+
+
+  -- replace hJ := hJ.basis_cl_right
+  -- rw []
+
+  -- rw [← hJ.subset.antisymm]
+  -- · exact hJ.indep
+  -- rintro e ⟨_, ⟨i₀,_, rfl⟩, (hei₀ : e ∈ Js i₀)⟩
+
+
+
+
 
 --   -- obtain ⟨I₀, hI₀⟩ := (hC.diff_singleton_indep heC).subset_basis_of_subset (subset_union_left _ (Js i₀))
 
